checkpoint before allowing sequential composition of non-atomic probe actions

src/3d/Generate32BitTypes.fst
@@ -26,25 +26,6 @@ module H = Hashtable
 module B = Binding
 open GlobalEnv
 
-//only specializing pointer types to 32 bit
-let rec maybe_specialize_32 (t:typ)
-: option typ
-= match t.v with
-  | Pointer t0 pq -> (
-    let t0' = maybe_specialize_32 t0 in
-    match pq, t0' with
-    | PQ UInt32, None ->
-      None
-    | _, _ ->
-      let t0 = 
-        match t0' with
-        | None -> t0
-        | Some t0' -> t0'
-      in
-      Some tuint32
-  )
-  | _ -> None
-
 let name32 (head_name:ident) : ident =
   let gen = reserved_prefix ^ "specialized32_" ^ head_name.v.name in
   {head_name with v = { head_name.v with name = gen }}
@@ -60,6 +41,33 @@ let gen_name_32 (n:typedef_names)
     typedef_abbrev = abbrev;
     typedef_ptr_abbrev = None;
     typedef_attributes = Noextract :: List.filter Aligned? n.typedef_attributes }
+
+//only specializing pointer types to 32 bit
+let rec maybe_specialize_32 (e:B.env) (t:typ)
+: ML (option typ)
+= match t.v with
+  | Pointer t0 pq -> (
+    let t0' = maybe_specialize_32 e t0 in
+    match pq, t0' with
+    | PQ UInt32, None ->
+      None
+    | _, _ ->
+      let t0 = 
+        match t0' with
+        | None -> t0
+        | Some t0' -> t0'
+      in
+      Some tuint32
+  )
+  | Type_app id ts gs ps -> (
+    let t = B.unfold_typ_abbrev_and_enum e t in
+    if B.typ_is_integral e t
+    then None
+    else (
+      Some { t with v = Type_app (name32 id) ts gs ps }
+    )
+  )
+  | _ -> None
 
 let maybe_gen_l 
       (gen_a: ('a -> ML (bool & 'a)))
@@ -78,50 +86,50 @@ let maybe_gen_l
   else false, l
   
 
-let rec gen_field (f:field) 
+let rec gen_field (e:B.env) (f:field) 
 : ML (bool & field)
 = match f.v with
   | AtomicField af -> (
-    match maybe_specialize_32 af.v.field_type with
+    match maybe_specialize_32 e af.v.field_type with
     | None -> false, f
     | Some t32 ->
       let af32 = { af with v = { af.v with field_type = t32; field_probe=None } } in
       true, { f with v=AtomicField af32 }
   )
   | RecordField r i -> (
-    let changed, r' = maybe_gen_l gen_field r in
+    let changed, r' = maybe_gen_l (gen_field e) r in
     if changed
     then true, { f with v=RecordField r' i }
     else false, f
   )
   | SwitchCaseField sw i -> (
-    let changed, cases = maybe_gen_l gen_case (snd sw) in
+    let changed, cases = maybe_gen_l (gen_case e) (snd sw) in
     let sw = (fst sw, cases) in
     if changed
     then true, { f with v=SwitchCaseField sw i }
     else false, f
   )
 
-and gen_case (c:case)
+and gen_case (env:B.env) (c:case)
 : ML (bool & case)
 = match c with
   | Case e f -> (
-    let b, f' = gen_field f in
+    let b, f' = gen_field env f in
     if b
     then b, Case e f'
     else false, c
   )
   | DefaultCase f -> (
-    let b, f' = gen_field f in
+    let b, f' = gen_field env f in
     if b
     then b, DefaultCase f'
     else false, c
   )
 
-let rec gen_decl (e:Binding.env) (d:decl) : ML (option decl) =
+let rec gen_decl (env:Binding.env) (d:decl) : ML (option decl) =
   match d.d_decl.v with
   | Record names gs params w fields ->
-    let changed, fields32 = maybe_gen_l gen_field fields in
+    let changed, fields32 = maybe_gen_l (gen_field env) fields in
     if changed
     then (
       let names_32 = gen_name_32 names in
@@ -131,7 +139,7 @@ let rec gen_decl (e:Binding.env) (d:decl) : ML (option decl) =
     else None
 
   | CaseType names gs params (e, cases) -> (
-    let changed, cases = maybe_gen_l gen_case cases in
+    let changed, cases = maybe_gen_l (gen_case env) cases in
     if changed
     then (
       let names_32 = gen_name_32 names in
@@ -144,8 +152,8 @@ let rec gen_decl (e:Binding.env) (d:decl) : ML (option decl) =
   | TypeAbbrev attrs t i gs ps -> (
     match t.v with
     | Type_app id _ _ _ -> (
-      let decl, _ = Binding.lookup_type_decl e id in
-      gen_decl e decl
+      let decl, _ = Binding.lookup_type_decl env id in
+      gen_decl env decl
       ) 
     | _ -> None
   )
@@ -163,7 +171,12 @@ let gen_decls (e:Binding.env) (d: decl)
       let c = mk_decl c d.d_decl.range [] false in
       [d;c]
     | Some d' ->
-      let src::_ = idents_of_decl d' in
+      let src =
+        match idents_of_decl d' with
+        | [id] -> id
+        | [_; id] -> id
+        | _ -> failwith "Unexpected number of names"
+      in
       let name = name32 id in
       let c =
         mk_decl 
@@ -176,6 +189,17 @@ let gen_decls (e:Binding.env) (d: decl)
   )
   | _ ->
     [d]
+
+let has_32bit_coercion (e:B.env) (t32 t:typ) : ML (option ident) =
+  let t32 = B.unfold_typ_abbrev_only e t32 in
+  let t = B.unfold_typ_abbrev_only e t in
+  match t.v, t32.v with
+  | Type_app id _ _ _, Type_app id32 _ _ _ -> 
+    FStar.IO.print_string <|
+      Printf.sprintf "Checking for coercion from %s to %s\n" (print_ident id32) (print_ident id);
+    GlobalEnv.find_probe_fn (B.global_env_of_env e) (CoerceProbeFunction (id32, id))
+  | _ ->
+    None
 
 let generate_32_bit_types (e:GlobalEnv.global_env) (d: list decl)
 : ML (list decl)
